src/Prototype/MostBasic.v
@@ -254,3 +254,7 @@ Section Impl.
 
 End Impl.
 
+Theorem impl_serial: SerialObjects svm_is_req impl.
+Proof.
+Admitted.
+
